QS.v
@@ -7,7 +7,9 @@ Record qs_dfa {A B} := {
   g : @dfa A B;
   n0 : Z;
   n : Z;
+  n1 : Z;
   n_correct : n >= n0;
+  n1_correct : n1 <= n0;
   count_event : B -> Z
 }.
 
@@ -33,6 +35,17 @@ Lemma count_buffer_distr' w e :
   count_buffer (w ++ [e]) = count_buffer w + (count_event qs e).
 Proof.
   rewrite count_buffer_distr; simpl; omega.
+Qed.
+
+Theorem count_word_pow: forall w n,
+  count_buffer (word_pow B w n) = (Z.of_nat n) * (count_buffer w).
+Proof.
+  intros w n.
+  induction n as [|n IH]. auto.
+  replace (word_pow B w (S n)) with (w ++ word_pow B w n).
+  rewrite count_buffer_distr, IH, Nat2Z.inj_succ, <- Zmult_succ_l_reverse;
+  omega.
+  auto.
 Qed.
 
 End QS.
